%\documentclass[UTF8]{ctexart} % use larger type; default would be 10pt
\documentclass[a4paper]{article}
\usepackage{xeCJK}
%\usepackage[utf8]{inputenc} % set input encoding (not needed with XeLaTeX)

%%% Examples of Article customizations
% These packages are optional, depending whether you want the features they provide.
% See the LaTeX Companion or other references for full information.

%%% PAGE DIMENSIONS
\usepackage{geometry} % to change the page dimensions
\geometry{a4paper} % or letterpaper (US) or a5paper or....
\geometry{margin=1in} % for example, change the margins to 2 inches all round
% \geometry{landscape} % set up the page for landscape
%   read geometry.pdf for detailed page layout information

\usepackage{graphicx} % support the \includegraphics command and options

% \usepackage[parfill]{parskip} % Activate to begin paragraphs with an empty line rather than an indent

%%% PACKAGES
\usepackage{booktabs} % for much better looking tables
\usepackage{array} % for better arrays (eg matrices) in maths
\usepackage{paralist} % very flexible & customisable lists (eg. enumerate/itemize, etc.)
\usepackage{verbatim} % adds environment for commenting out blocks of text & for better verbatim
\usepackage{subfig} % make it possible to include more than one captioned figure/table in a single float
% These packages are all incorporated in the memoir class to one degree or another...

%%% HEADERS & FOOTERS
\usepackage{fancyhdr} % This should be set AFTER setting up the page geometry
\pagestyle{fancy} % options: empty , plain , fancy
\renewcommand{\headrulewidth}{0pt} % customise the layout...
\lhead{}\chead{}\rhead{}
\lfoot{}\cfoot{\thepage}\rfoot{}

%%% SECTION TITLE APPEARANCE
\usepackage{sectsty}
\allsectionsfont{\sffamily\mdseries\upshape} % (See the fntguide.pdf for font help)
% (This matches ConTeXt defaults)

%%% ToC (table of contents) APPEARANCE
\usepackage[nottoc,notlof,notlot]{tocbibind} % Put the bibliography in the ToC
\usepackage[titles,subfigure]{tocloft} % Alter the style of the Table of Contents
\renewcommand{\cftsecfont}{\rmfamily\mdseries\upshape}
\renewcommand{\cftsecpagefont}{\rmfamily\mdseries\upshape} % No bold!

%%% END Article customizations

%%% The "real" document content comes below...

\setlength{\parindent}{0pt}
\usepackage{physics}
\usepackage{amsmath}
%\usepackage{symbols}
\usepackage{AMSFonts}
\usepackage{bm}
%\usepackage{eucal}
\usepackage{mathrsfs}
\usepackage{amssymb}
\usepackage{float}
\usepackage{multicol}
\usepackage{abstract}
\usepackage{empheq}
\usepackage{extarrows}
\usepackage{textcomp}
\usepackage{fontspec}
\usepackage{braket}
\usepackage{siunitx}
\sisetup{
	separate-uncertainty = true,
	inter-unit-product = \ensuremath{{}\cdot{}}
}

\DeclareMathOperator{\p}{\prime}
\DeclareMathOperator{\ti}{\times}
\DeclareMathOperator{\intinf}{\int_0^\infty}
\DeclareMathOperator{\intdinf}{\int_{-\infty}^\infty}
\DeclareMathOperator{\intzpi}{\int_0^\pi}
\DeclareMathOperator{\intztpi}{\int_0^{2\pi}}
\DeclareMathOperator{\suminf}{\sum_{n=1}^{\infty}}
\DeclareMathOperator{\suminfz}{\sum_{n=0}^\infty}
\DeclareMathOperator{\sumkinf}{\sum_{k=1}^{\infty}}
\DeclareMathOperator{\sumkinfz}{\sum_{k=0}^\infty}
\DeclareMathOperator{\e}{\mathrm{e}}
\DeclareMathOperator{\I}{\mathrm{i}}
\DeclareMathOperator{\Arg}{\mathrm{Arg}}
\DeclareMathOperator{\ra}{\rightarrow}
\DeclareMathOperator{\llra}{\longleftrightarrow}
\DeclareMathOperator{\lra}{\longrightarrow}
\DeclareMathOperator{\dlra}{\Leftrightarrow}
\DeclareMathOperator{\dra}{\Rightarrow}
\newcommand{\bkk}[1]{\Braket{#1|#1}}
\newcommand{\bk}[2]{\Braket{#1|#2}}
\newcommand{\bkev}[2]{\Braket{#2|#1|#2}}



\DeclareMathOperator{\hV}{\hat{\vb{V}}}

\DeclareMathOperator{\hx}{\hat{\vb{x}}}
\DeclareMathOperator{\hy}{\hat{\vb{y}}}
\DeclareMathOperator{\hz}{\hat{\vb{z}}}

\DeclareMathOperator{\hA}{\hat{\vb{A}}}

\DeclareMathOperator{\hQ}{\hat{\vb{Q}}}
\DeclareMathOperator{\hI}{\hat{\vb{I}}}
\DeclareMathOperator{\psis}{\psi^\ast}
\DeclareMathOperator{\Psis}{\Psi^\ast}
\DeclareMathOperator{\hi}{\hat{\vb{i}}}
\DeclareMathOperator{\hj}{\hat{\vb{j}}}
\DeclareMathOperator{\hk}{\hat{\vb{k}}}
\DeclareMathOperator{\hr}{\hat{\vb{r}}}
\DeclareMathOperator{\hT}{\hat{\vb{T}}}
\DeclareMathOperator{\hH}{\hat{H}}
\DeclareMathOperator{\hh}{\hat{h}}               % helicity
\DeclareMathOperator{\hL}{\hat{\vb{L}}}
\DeclareMathOperator{\hp}{\hat{\vb{p}}}

\DeclareMathOperator{\ha}{\hat{\vb{a}}}
\DeclareMathOperator{\hS}{\hat{\vb{S}}}
\DeclareMathOperator{\hSigma}{\hat{\bm\Sigma}}
\DeclareMathOperator{\hJ}{\hat{\vb{J}}}
\DeclareMathOperator{\hP}{\hat{\vb{P}}}          % Parity
\DeclareMathOperator{\hC}{\hat{\vb{C}}} 
\DeclareMathOperator{\Tdv}{-\dfrac{\hbar^2}{2m}\dv[2]{x}}
\DeclareMathOperator{\Tna}{-\dfrac{\hbar^2}{2m}\nabla^2}
\DeclareMathOperator{\vna}{\vnabla}
\DeclareMathOperator{\nna}{\nabla^2}
\newcommand{\naCarExpd}[1]{\pdv[2]{#1}{x} + \pdv[2]{#1}{y} + \pdv[2]{#1}{z}}
\newcommand{\naCyl}{\qty[\dfrac{1}{\rho}\pdv{\rho}\qty(\rho\pdv{\rho}) + \dfrac{1}{\rho^2}\pdv[2]{\phi} + \pdv[2]{z}]}

%\DeclareMathOperator{\g#0}{\gamma^0}
%\DeclareMathOperator{\g1}{\gamma^1}
%\DeclareMathOperator{\g2}{\gamma^2}
%\DeclareMathOperator{\g3}{\gamma^3}
%\DeclareMathOperator{\g5}{\gamma^5}
\newcommand{\g}[1]{\gamma^{#1}}
\DeclareMathOperator{\gmuu}{\gamma^\mu}
\DeclareMathOperator{\gmud}{\gamma_\mu}
\newcommand{\G}[2]{g^{#1#2}}

\newcommand{\subsbul}{\subsection*{$ \bullet $}}
\newcommand{\ex}[1]{\paragraph{Ex #1}}
\newcommand{\subex}[1]{\subparagraph{#1}}
\newcommand{\dis}{\displaystyle}
\newcommand{\iden}{{\large \bm{1}}}
\newcommand{\qed}{$ \Square $}
\numberwithin{equation}{subsection}
%\allowdisplaybreaks[4]

\title{\textbf{Modern Quantum Chemistry, Szabo \& Ostlund}\\HW}
\author{王石嵘
\vspace{5pt}\\
%161240065\\
%Email: shirong\_wang@berkeley.edu
}
\date{\today} % Activate to display a given date or no date (if empty),
         % otherwise the current date is printed 

\begin{document}
% \boldmath

\maketitle

\tableofcontents

\newpage

%\setcounter{section}{1}
\section{Mathematical Review}
\subsection{Linear Algebra}
\subsubsection{3-D Vector Algebra}
\ex{1.1}
\subex{a)}
\begin{equation}\label{key}
\mathcal{O}\vb{e}_j = \sum_{i=1}^3 \vb{e}_i O_{ij}
\end{equation}
\begin{equation}\label{key}
\vb{e}_i \cdot \mathcal{O}\vb{e}_j = \vb{e}_i \cdot \sum_{i=1}^3 \vb{e}_i O_{ij} = O_{ij}
\end{equation}
\subex{b)}
\begin{equation}\label{key}
\begin{aligned}
\vb{b} &= \mathcal{O}\vb{a} = \sum_{i=1}^3 a_i\sum_{j=1}^3 \vb{e}_jO_{ji}\\
&=\sum_{j=1}^3 a_j\sum_{i=1}^3 \vb{e}_iO_{ij} = \sum_{i=1}^3 \vb{e}_i\sum_{j=1}^3 a_jO_{ij}
\end{aligned}
\end{equation}
thus
\begin{equation}\label{key}
\vb{b}_i = \sum_{j=1}^3 a_jO_{ij}
\end{equation}

\ex{1.2}
\begin{equation}\label{key}
[\vb{A},\vb{B}] = \mqty[0& -2& 4\\2& 0& 3\\-4& -3& 0]
\end{equation}
\begin{equation}\label{key}
\{\vb{A},\vb{B}\} = \mqty[0& 0& -2\\0& -2& 3\\-2& 3& -2]
\end{equation}

\subsubsection{Matrices}
\ex{1.3}
\begin{equation}\label{key}
(AB)_{nk} = \sum_m^M A_{nm}B_{mk}
\end{equation}
\begin{equation}\label{key}
(AB)^\dagger_{kn} = (AB)_{nk}^* = \sum_m^M A_{nm}^*B_{mk}^* = \sum_m^M B^\dagger_{km} A^\dagger_{mn} = (B^\dagger A^\dagger)_{kn}
\end{equation}
thus
\begin{equation}\label{key}
(\vb{A}\vb{B})^\dagger = \vb{B}^\dagger \vb{A}^\dagger
\end{equation}

\ex{1.4}
\subex{a.}
suppose $ \vb{A} $ is $ N\cross M $ and $ \vb{B} $ is $ M\cross N $
\begin{equation}\label{key}
\tr \vb{A}\vb{B} = \sum_n^N (AB)_{nn} = \sum_n^N \sum_m^M A_{nm}B_{mn} = \sum_m^M\sum_n^N  B_{mn}A_{nm} = \sum_m^M (BA)_{mm} = \tr \vb{B}\vb{A}
\end{equation}
\subex{b.}
\begin{equation}\label{key}
\vb{AB}(\vb{AB})^{-1} = \iden
\end{equation}
\begin{equation}\label{key}
\vb{B}^{-1}\vb{A}^{-1}\vb{A}\vb{B}(\vb{AB})^{-1} = \vb{B}^{-1}\vb{A}^{-1}\iden
\end{equation}
\begin{equation}\label{key}
\vb{B}^{-1}(\vb{A}^{-1}\vb{A})\vb{B}(\vb{AB})^{-1} = \vb{B}^{-1}\vb{A}^{-1}
\end{equation}
\begin{equation}\label{key}
\vb{B}^{-1} \iden \vb{B}(\vb{AB})^{-1} = \vb{B}^{-1}\vb{A}^{-1}
\end{equation}
thus
\begin{equation}\label{key}
(\vb{AB})^{-1} = \vb{B}^{-1}\vb{A}^{-1}
\end{equation}
\subex{c.}
\begin{equation}\label{key}
\vb{B} = \vb{U}^\dagger \vb{A} \vb{U}
\end{equation}huhhj
\begin{equation}\label{key}
\vb{U} \vb{B} \vb{U}^\dagger = \vb{U} \vb{U}^\dagger \vb{A} \vb{U} \vb{U}^\dagger = \iden \vb{A} \iden = \vb{A}
\end{equation}
\subex{d.}
$ \because \vb{C}$ is Hermitian, $ \therefore $
\begin{equation}\label{key}
\vb{C} = \vb{C}^\dagger
\end{equation}
\begin{equation}\label{key}
\vb{A}\vb{B} = (\vb{A}\vb{B})^\dagger = \vb{B}^\dagger \vb{A}^\dagger
\end{equation}
Since $ \vb{A} $, $ \vb{B} $ are Hermitian,
\begin{equation}\label{key}
\vb{A}\vb{B} = \vb{B}^\dagger \vb{A}^\dagger = \vb{B}\vb{A}
\end{equation}
$ \therefore $
\begin{equation}\label{key}
[\vb{A}, \vb{B}] = \vb{A}\vb{B} - \vb{B}\vb{A} = 0
\end{equation}
i.e. $ \vb{A} $, $ \vb{B} $ commute
\subex{e.}
Since $ \vb{A} $ is Hermitian,
\begin{equation}\label{key}
\vb{A} = \vb{A}^\dagger
\end{equation}
thus
\begin{equation}\label{key}
(\vb{A}^{1-})^\dagger \vb{A} = (\vb{A}^{1-})^\dagger \vb{A}^\dagger = (\vb{A}\vb{A}^{-1})^\dagger = \iden^\dagger = \iden
\end{equation}
thus
\begin{equation}\label{key}
(\vb{A}^{1-})^\dagger \vb{A} \vb{A}^{-1} = \vb{A}^{-1}
\end{equation}
\begin{equation}\label{key}
(\vb{A}^{1-})^\dagger = \vb{A}^{-1}
\end{equation}
i.e. $ \vb{A}^{-1} $, if it exists, is Hermitian.
\subex{f.}
Suppose
\begin{equation}\label{key}
\vb{A}^{-1} = \mqty(x & y\\z & w)
\end{equation}
thus
\begin{equation}\label{key}
\mqty(A_{11} & A_{12}\\A_{21} & A_{22})\mqty(x & y\\z & w) = \mqty(1 & 0\\0 & 1)
\end{equation}
the solution is
\begin{equation}\label{key}
\mqty{
	&x = \dfrac{A_{22}}{A_{11}A_{22} - A_{12}A_{21}}\\
	&y = \dfrac{-A_{12}}{A_{11}A_{22} - A_{12}A_{21}}\\
	&z = \dfrac{-A_{21}}{A_{11}A_{22} - A_{12}A_{21}}\\
	&w = \dfrac{A_{11}}{A_{11}A_{22} - A_{12}A_{21}}\\ 
}
\end{equation}
thus
\begin{equation}\label{key}
\vb{A}^{-1} = \dfrac{1}{\det(\vb{A})} \mqty(A_{22} & -A_{12}\\ -A_{21} & A_{11})
\end{equation}

\subsubsection{Determinants}
\ex{1.5}
Suppose 
\begin{equation}\label{key}
\vb{A} = \mqty(A_{11} & A_{12}\\A_{21} & A_{22})
\end{equation}
\subex{1.}
\begin{equation}\label{key}
\mqty|0 & 0\\A_{21} & A_{22}| = 0\cdot A_{22} - 0\cdot A_{21} = 0
\end{equation}
\begin{equation}\label{key}
\mqty|0 & A_{12}\\0 & A_{22}| = 0\cdot A_{22} - 0\cdot A_{12} = 0
\end{equation}
\subex{2.}
\begin{equation}\label{key}
\det(\vb{A}) = A_{11}A_{22} -  0\cdot 0 = A_{11}A_{22}
\end{equation}
\subex{3.}
\begin{equation}\label{key}
\det(\vb{A}) = A_{11}A_{22} -  A_{12}A_{21}
\end{equation}
\begin{equation}\label{key}
\mqty| A_{21} & A_{22}\\A_{11} & A_{12} | = A_{21}A_{12} - A_{22}A_{11} = -\det(\vb{A})
\end{equation}
\subex{4.}
\begin{equation}\label{key}
\det(\vb{A}^\dagger)^* = \mqty|A_{11}^* & A_{21}^*\\A_{12}^* & A_{22}^*|^* = (A_{11}^*A_{22}^* - A_{21}^*A_{12}^*)^* = A_{11}A_{22} -  A_{12}A_{21} = \det(\vb{A})
\end{equation}
\subex{5.}
Suppose $ \vb{B} = \mqty(B_{11} & B_{12}\\B_{21} & B_{22}) $
\begin{equation}\label{key}
\begin{aligned}
\det(\vb{A}\vb{B}) &= 
\mqty|A_{11}B_{11}+A_{12}B_{21} & A_{11}B_{12}+A_{12}B_{22}\\
A_{21}B_{11}+A_{22}B_{21} & A_{21}B_{12}+A_{22}B_{22}|\\
&= (A_{11}B_{11}+A_{12}B_{21})(A_{21}B_{12}+A_{22}B_{22}) - (A_{11}B_{12}+A_{12}B_{22})(A_{21}B_{11}+A_{22}B_{21})\\
&= A_{11}B_{11}A_{21}B_{12} + A_{11}B_{11}A_{22}B_{22} + A_{12}B_{21}A_{21}B_{12} + A_{12}B_{21}A_{22}B_{22}\\
&\quad - (A_{11}B_{12}A_{21}B_{11} +  A_{11}B_{12}A_{22}B_{21} + A_{12}B_{22}A_{21}B_{11} + A_{12}B_{22}A_{22}B_{21})\\
&= A_{11}B_{11}A_{22}B_{22} + A_{12}B_{21}A_{21}B_{12} - A_{11}B_{12}A_{22}B_{21} - A_{12}B_{22}A_{21}B_{11}
\end{aligned}
\end{equation}
\begin{equation}\label{key}
\begin{aligned}
\det(\vb{A})\det(\vb{B}) &= (A_{11}A_{22} -  A_{12}A_{21})(B_{11}B_{22} -  B_{12}B_{21})\\
&= A_{11}A_{22}B_{11}B_{22} - A_{11}A_{22}B_{12}B_{21} - A_{12}A_{21}B_{11}B_{22} + A_{12}A_{21}B_{12}B_{21}\\
&= A_{11}B_{11}A_{22}B_{22} + A_{12}B_{21}A_{21}B_{12}- A_{11}B_{12}A_{22}B_{21} - A_{12}B_{22}A_{21}B_{11} \\
\end{aligned}
\end{equation}
$ \therefore $
\begin{equation}\label{key}
\det(\vb{A})\det(\vb{B}) = \det(\vb{A}\vb{B})
\end{equation}

\ex{1.6}
\subex{6.}
If two rows (e.g. $ i $th and $ j $th) are equal
\begin{equation}\label{key}
\det(\vb{A}) = \mqty|  & ... & ... & \\
      A_{i1} & A_{i2} & ... & A_{in}\\
        & ... & ... & \\
      A_{j1} & A_{j2} & ... & A_{jn}\\
        & ... & ... & \\|
\xlongequal{1.5.3} -\mqty|  & ... & ... & \\
A_{j1} & A_{j2} & ... & A_{jn}\\
& ... & ... & \\
A_{i1} & A_{i2} & ... & A_{in}\\
& ... & ... & \\|
= - \mqty|  & ... & ... & \\
A_{i1} & A_{i2} & ... & A_{in}\\
& ... & ... & \\
A_{j1} & A_{j2} & ... & A_{jn}\\
& ... & ... & \\|
\end{equation}
i.e.
\begin{equation}\label{key}
\det(\vb{A}) = -\det(\vb{A})
\end{equation}
thus
\begin{equation}\label{key}
\det(\vb{A}) = 0
\end{equation}
\subex{7.}
From Ex 1.5.5, we have
\begin{equation}\label{key}
\det(\vb{A})\det(\vb{A}^{-1}) = \det(\iden) = 1
\end{equation}
thus
\begin{equation}\label{key}
\det(\vb{A}^{-1}) = \det(\vb{A})^{-1}
\end{equation}
\subex{8.}
\begin{equation}\label{key}
\vb{A}\vb{A}^\dagger = \iden \;\dra\; \det(\vb{A})\det(\vb{A}^\dagger) = \det(\iden) = 1
\end{equation}
From Ex 1.5.4, we have
\begin{equation}\label{key}
\det(\vb{A})\det(\vb{A})^* = 1
\end{equation}
\subex{9.}
From Ex 1.5.5, we get
\begin{equation}\label{key}
\det(\vb{U}^\dagger)\det(\vb{O})\det(\vb{U}) = \det(\bm\Omega)
\end{equation}
and
\begin{equation}\label{key}
\det(\vb{U}^\dagger)\det(\vb{U}) = \det(\iden) = 1
\end{equation}
$ \therefore $
\begin{equation}\label{key}
\det(\vb{O}) = \det(\bm\Omega)
\end{equation}

\ex{1.7}
If $ \det(\vb{A}) \neq 0 $, thus $ \vb{A}^{-1} $ exists, we have
\begin{equation}\label{key}
\vb{A}^{-1}\vb{A}\vb{c} = \bm{0} \;\dra\; \vb{c} = \bm{0}
\end{equation}
$  \square $

\subsubsection{N-D Complex Vector Spaces}

\subsubsection{Change of Basis}
\ex{1.8}
\begin{equation}\label{key}
\Omega_{\alpha\beta} = \sum_{ij} U_{\alpha i}^\dagger O_{ij} U_{j\beta}
\end{equation}
gives
\begin{equation}\label{key}
\begin{aligned}
\tr\bm\Omega &= \sum_\alpha \Omega_{\alpha\alpha} = \sum_\alpha \sum_{ij} U_{\alpha i}^\dagger O_{ij} U_{j\alpha}\\
&= \sum_{ij} O_{ij} \sum_\alpha U_{j\alpha} U_{\alpha i}^\dagger = \sum_{ij} O_{ij} \delta_{ji} = \tr\vb{O}
\end{aligned}
\end{equation}
%while
%\begin{equation}\label{key}
%O_{ij} = \sum_{\alpha\beta} U_{i\alpha} \Omega_{\alpha\beta} U_{\beta j}^\dagger
%\end{equation}
%gives
%\begin{equation}\label{key}
%\tr \vb{O} = \sum_{i} O_{ii} = \sum_{\alpha\beta} U_{i\alpha} \Omega_{\alpha\beta} U_{i\beta}^*
%\end{equation}

\subsubsection{The Eigenvalue Problem}
\ex{1.9}
\begin{equation}\label{key}
\vb{O}\vb{U} = \vb{U}\bm\omega \;\dra\; \vb{O}\mqty(\vb{c}^1 & \vb{c}^2 & \cdots & \vb{c}^N) = \mqty(\omega_1\vb{c}_1 & \omega_2\vb{c}_2 & \cdots & \omega_N\vb{c}_N)
\end{equation}
thus
\begin{equation}\label{key}
\vb{O}\vb{c}^\alpha = \omega_\alpha \vb{c}^\alpha
\end{equation}
\ex{1.10}
\begin{equation}\label{key}
\left\{
\begin{aligned}
&O_{11}-\omega + O_{12}c = 0\\
&O_{21} + (O_{22}-\omega)c = 0
\end{aligned}\right.
\end{equation}
\begin{equation}\label{key}
(O_{11}-\omega)(O_{22}-\omega) - O_{21}O_{12} = 0
\end{equation}
\begin{equation}\label{key}
\omega^2 - (O_{11}+O_{22})\omega + O_{11}O_{22} - O_{21}O_{12} = 0
\end{equation}
\begin{equation}\label{key}
\left\{\begin{aligned}
&\omega_1 = \dfrac{1}{2}\qty(O_{11}+O_{22} - \sqrt{(O_{11}-O_{22})^2 + 4O_{21}O_{12}})\\
&\omega_2 = \dfrac{1}{2}\qty(O_{11}+O_{22} + \sqrt{(O_{11}-O_{22})^2 + 4O_{21}O_{12}})
\end{aligned}\right.
\end{equation}
\ex{1.11}

\end{document}